

# Number Theory Exercises

(solutions at the end)

- ① Find all  $n \in \mathbb{N}$  with  $n \geq 1$  and  $(n+1) \mid (n^2+1)$ .  
From the book "250 problems in elementary number theory"

Option 1: • Remember the definition of  $x \mid y$   
• for all  $x, y$  either  $x < y$ ,  $x = y$  or  $x > y$

Option 2: • Remember that  $a+0=a$  and  $0=n-n$

- ② Prove that  $\gcd(a, \gcd(b, c)) = \gcd(\gcd(a, b), c)$

Hint: Use the prime number definition of  $\gcd$ .

- ③ (\*) Compute the set of solutions  $(x, y) \in \mathbb{Z}_{11} \times \mathbb{Z}_{11}$  to the congruence system

$$2x + 9y \equiv_{11} 7$$

$$2x + 7y \equiv_{11} 5$$

$$4x + 5y \equiv_{11} 1.$$

From the HS24 exam.

Hint: Just treat them like you treated normal equations in school.

- ④ (\*) Consider the polynomial  $f(x) = x^4 + x^2 + 1$ . Prove that: for all primes  $p \in \mathbb{Z}$ , the evaluation  $f(p)$  is **not** prime. (4 Points)

From the HS24 exam.

Option 1: • Remember that each number is either  $3k+0$ ,  $3k+1$  or  $3k+2$  for some  $k$ .  
So  $x \equiv_3 0$  or  $x \equiv_3 1$  or  $x \equiv_3 2$ .

Option 2: • Remember that  $0 = x^2 - x^2$   
• Remember that  $(a+b)^2 = a^2 + 2ab + b^2$   
• Remember that  $a^2 - b^2 = (a-b)(a+b)$

## SOLUTIONS:

① Option 1: Say that  $n+1 \mid n^2+1$ . Then there exists  $x$  such that  $x(n+1) = n^2+1$ .

Now we do a case distinction:

a)  $x > n$ : Then  $x(n+1) > n(n+1) = n^2+n$ .

This means  $n^2+1 > n^2+n$

$\Rightarrow 1 > n$ , but we want  $n \geq 1$

b)  $x < n$ : Then  $x \leq n-1$  and  $x(n+1) \leq (n-1)(n+1) = n^2-1$ .

This means  $n^2+1 \leq n^2-1$

$\Rightarrow 1 \leq -1$ , a contradiction

c)  $x = n$ : Then  $x(n+1) = n(n+1) = n^2+n$ .

This means  $n^2+n = n^2+1$

$\Rightarrow n = 1$

So 1 is the only solution.

Option 2: We use the fact that  $n - n = 0$ :

$$n^2+1 = n^2+1+0 = n^2+1+n-n = n^2+n-(n-1) = n(n+1)-(n-1)$$

So if  $(n+1) \mid (n^2+1)$  then  $(n+1) \mid (n-1)$ , since it already divides  $n(n+1)$ . But since  $n+1 > n-1$  this only holds for  $n-1 = 0$  and so only for  $n = 1$ .

② Say  $a = \prod_i p_i^{\alpha_i}$ ,  $b = \prod_i p_i^{\beta_i}$ ,  $c = \prod_i p_i^{\gamma_i}$ .

Then  $\gcd(b, c) = \prod_i p_i^{\min(\beta_i, \gamma_i)}$ .

And so  $\gcd(a, \gcd(b, c)) = \prod_i p_i^{\min(\alpha_i, \min(\beta_i, \gamma_i))}$ .

A similar argument shows that  $\gcd(\gcd(a, b), c) = \prod_i p_i^{\min(\min(\alpha_i, \beta_i), \gamma_i)}$ .

To show that they are equal we show that:

$$\min(x, \min(y, z)) = \min(\min(x, y), z) \quad \text{for all } x, y, z.$$

We do a case distinction:

a)  $x \leq y \wedge x \leq z$ : Then  $x \leq \min(y, z)$  since  $\min(y, z)$  is either  $y$  or  $z$  and so the LHS is  $x$ .  
Also  $\min(x, y) = x$  and  $\min(x, z) = x$  so the RHS is also  $x$ .

b)  $y \leq x \wedge y \leq z$

c)  $z \leq x \wedge z \leq y$  follow similar arguments.

Since we can order the numbers, one of them has to be first in the ordering, so one of the cases must apply.

We showed that  $\min(\alpha_i, \min(\beta_i, \gamma_i)) = \min(\min(\alpha_i, \beta_i), \gamma_i)$

$$\Rightarrow \prod_i p_i^{\min(\alpha_i, \min(\beta_i, \gamma_i))} = \prod_i p_i^{\min(\min(\alpha_i, \beta_i), \gamma_i)}$$

$$\Rightarrow \gcd(a, \gcd(b, c)) = \gcd(\gcd(a, b), c)$$

We showed that the magma  $(\mathbb{N}, \gcd)$  is actually a semigroup!

$$\begin{aligned} \textcircled{3} \text{ We have } \quad 2x + 9y &\equiv_{11} 7 & \textcircled{1} \\ 2x + 7y &\equiv_{11} 5 & \textcircled{2} \\ 4x + 5y &\equiv_{11} 1 & \textcircled{3} \end{aligned}$$

Subtracting  $\textcircled{1}-\textcircled{2}$  gives  $2y \equiv_{11} 2$  and so  $y \equiv_{11} 1$ .

Substituting into  $\textcircled{3}$  gives  $4x + 5 \equiv_{11} 1$

$$\Rightarrow 4x \equiv_{11} -4$$

$$\Rightarrow x \equiv_{11} -1$$

$$\Rightarrow x \equiv_{11} 10 \quad (+11 \text{ on both sides})$$

So  $x = 10$  and  $y = 1$

$\textcircled{4}$

Option 1: We do a case distinction:

a)  $R_3(p) = 0$ . The only prime for which this holds is 3 (since if  $R_3(p) = 0$  then it is divisible by 3).

$$\text{We see that } f(3) = 3^4 + 3^2 + 1 = 81 + 9 + 1 = 91 = 7 \cdot 13$$

$$\begin{aligned} \text{b) } R_3(p) = 1. \text{ Then } R_3(f(p)) &= R_3(p^4 + p^2 + 1) \\ &= R_3(R_3(p)^4 + R_3(p)^2 + 1) \\ &= R_3(1^4 + 1^2 + 1) \\ &= R_3(3) = 0 \end{aligned}$$

and so  $f(p)$  is divisible by 3.

$$\begin{aligned} \text{c) } R_3(p) = 2. \text{ Then } R_3(f(p)) &= R_3(p^4 + p^2 + 1) \\ &= R_3(R_3(p)^4 + R_3(p)^2 + 1) \\ &= R_3(2^4 + 2^2 + 1) \\ &= R_3(16 + 4 + 1) \\ &= R_3(21) = 0 \end{aligned}$$

and so  $f(p)$  is divisible by 3.

In all cases  $f(p)$  is not a prime.

Fun fact: I managed to miscalculate one of the cases during the exam and tried until modulo 5 until I realized I was wasting time.

Option 2 by Jefferson Morales Morciano:

$$\begin{aligned} f(x) &= x^4 + x^2 + 1 \\ &= x^4 + x^2 + 1 + (x^2 - x^2) \\ &= x^4 + 2x^2 + 1 - x^2 \\ &= (x^2 + 1)^2 - x^2 \\ &= ((x^2 + 1) - x) \cdot ((x^2 + 1) + x) \end{aligned}$$

So it is a composite number, and therefore not prime.  
(Only for  $x=1$  we get  $f(1)=3$ , but 1 is not a prime.)